cfrontend/Cshmgenproof.v
@@ -1489,25 +1489,16 @@ Inductive match_states: Clight.state -> Csharpminor.state -> Prop :=
       match_states (Clight.State f s k e le m)
                    (State tf ts' tk' te le m)
   | match_callstate:
-<<<<<<< HEAD
-      forall vf fd args k m tfd tk targs tres cconv cu ce
+      forall vf fd args k m tfd tk targs tres cconv cu ce id
           (FS: Genv.find_funct ge vf = Some fd)
           (FT: Genv.find_funct tge vf = Some tfd)
-=======
-      forall fd args k m tfd tk targs tres cconv cu ce id
->>>>>>> origin/StackAware-new
           (LINK: linkorder cu prog)
           (TR: match_fundef cu fd tfd)
           (MK: match_cont ce tres 0%nat 0%nat k tk)
           (ISCC: Clight.is_call_cont k)
           (TY: type_of_fundef fd = Tfunction targs tres cconv),
-<<<<<<< HEAD
-      match_states (Clight.Callstate vf args k m)
-                   (Callstate vf args tk m)
-=======
-      match_states (Clight.Callstate fd args k m id)
-                   (Callstate tfd args tk m id)
->>>>>>> origin/StackAware-new
+      match_states (Clight.Callstate vf args k m id)
+                   (Callstate vf args tk m id)
   | match_returnstate:
       forall res tres k m tk ce
           (MK: match_cont ce tres 0%nat 0%nat k tk),
@@ -1698,13 +1689,8 @@ Proof.
                 sig_cc := cc |}) in *.
   assert (SIG: funsig tfd = sg).
   { unfold sg; erewrite typlist_of_arglist_eq by eauto.
-<<<<<<< HEAD
-    eapply transl_fundef_sig1; eauto. rewrite H3; auto. }
-(*  assert (EITHER: tk' = tk /\ ts' = Scall optid sg x x0).
-=======
     eapply transl_fundef_sig1; eauto. rewrite H4; auto. }
-  assert (EITHER: tk' = tk /\ ts' = Scall optid sg x x0
->>>>>>> origin/StackAware-new
+(*  assert (EITHER: tk' = tk /\ ts' = Scall optid sg x x0).
                \/ exists id, optid = Some id /\
                   tk' = tk /\ ts' = Sseq (Scall optid sg x x0)
                                          (Sset id (make_normalization tres (Evar id)))).
@@ -1713,13 +1699,9 @@ Proof.
     inv MTR. right; exists i; auto.
     inv MTR; auto.
     inv MTR; auto. }
-<<<<<<< HEAD
   destruct EITHER as [(EK & ES) | (id & EI & EK & ES)]; rewrite EK, ES.
   *)
   unfold make_funcall in MTR. inv MTR.
-=======
-  destruct EITHER as [(EK & ES) | (id' & EI & EK & ES)]; rewrite EK, ES.
->>>>>>> origin/StackAware-new
   + (* without normalization of return value *)
     econstructor; split.
     apply plus_one. eapply step_call; eauto.
@@ -1903,12 +1885,8 @@ Proof.
   econstructor; eauto. constructor.
 
 - (* internal function *)
-<<<<<<< HEAD
   rewrite FS in FIND. inv FIND.
-  inv H. inv TR. monadInv H5.
-=======
   inv H. inv TR. monadInv H6.
->>>>>>> origin/StackAware-new
   exploit match_cont_is_call_cont; eauto. intros [A B].
   exploit match_env_alloc_variables; eauto.
   apply match_env_empty.
@@ -1916,13 +1894,6 @@ Proof.
   econstructor; split.
   apply plus_one. eapply step_internal_function; eauto.
   simpl. erewrite transl_vars_names by eauto. assumption.
-<<<<<<< HEAD
-=======
-  simpl. assumption.
-  simpl. assumption.
-  eauto. eauto.
-  simpl; eauto.
->>>>>>> origin/StackAware-new
   simpl. rewrite create_undef_temps_match. eapply bind_parameter_temps_match; eauto.
   simpl. econstructor; eauto.
   unfold transl_function. rewrite EQ; simpl. rewrite EQ1; simpl. auto.
@@ -1937,11 +1908,7 @@ Proof.
   econstructor; split.
   apply plus_one. econstructor; eauto.
   eapply match_returnstate with (ce := ce); eauto.
-<<<<<<< HEAD
   (* apply has_rettype_wt_val. 
-=======
-  apply has_rettype_wt_val.
->>>>>>> origin/StackAware-new
   replace (rettype_of_type tres0) with (sig_res (ef_sig ef)).
   eapply external_call_well_typed_gen; eauto.
   rewrite H5. simpl. simpl in TY. congruence. *)
@@ -1966,7 +1933,6 @@ Lemma transl_initial_states:
   exists R, initial_state tge q R /\ match_states S R.
 Proof.
   intros. inv H.
-<<<<<<< HEAD
   exploit functions_translated; eauto. intros (cu & tf & A & B & C).
   eexists. split.
   - erewrite <- transl_fundef_sig2 by eauto. inv B. econstructor; eauto.
@@ -1984,17 +1950,6 @@ Proof.
   split. econstructor; eauto. intros r S' HS'. inv HS'.
   eexists. split. econstructor; eauto.
   econstructor; eauto.
-=======
-  exploit function_ptr_translated; eauto. intros (cu & tf & A & B & C).
-  assert (D: Genv.find_symbol tge (AST.prog_main tprog) = Some b).
-  { destruct TRANSL as (P & Q & R). rewrite Q. rewrite symbols_preserved. auto. }
-  assert (E: funsig tf = signature_of_type Tnil type_int32s cc_default).
-  { eapply transl_fundef_sig2; eauto. }
-  econstructor; split.
-  econstructor; eauto. apply (Genv.init_mem_match TRANSL). eauto.
-  destruct TRANSL as (P & Q & R). rewrite Q.
-  econstructor; eauto. instantiate (1 := prog_comp_env cu). constructor; auto. exact I.
->>>>>>> origin/StackAware-new
 Qed.
 
 Lemma transl_final_states:
@@ -2004,25 +1959,11 @@ Proof.
   intros. inv H0. inv H. inv MK. constructor.
 Qed.
 
-<<<<<<< HEAD
-=======
-Theorem transl_program_correct:
-  forward_simulation (Clight.semantics2 fn_stack_requirements prog)
-                     (Csharpminor.semantics fn_stack_requirements tprog).
-Proof.
-  eapply forward_simulation_plus.
-  apply senv_preserved.
-  eexact transl_initial_states.
-  eexact transl_final_states.
-  eexact transl_step.
-Qed.
-
->>>>>>> origin/StackAware-new
 End CORRECTNESS.
 
-Theorem transl_program_correct prog tprog:
+Theorem transl_program_correct fn_stack_requirements prog tprog:
   match_prog prog tprog ->
-  forward_simulation cc_id cc_id (Clight.semantics2 prog) (Csharpminor.semantics tprog).
+  forward_simulation cc_id cc_id (Clight.semantics2 fn_stack_requirements prog) (Csharpminor.semantics fn_stack_requirements tprog).
 Proof.
   fsim eapply forward_simulation_plus; cbn; destruct w, Hse.
   - intros q _ [ ]. eapply Genv.is_internal_match_id; eauto. destruct 1; auto.
